Full SHA-256 spec (#872)

silveroak-opentitan/hmac/Spec/SHA256.v
@@ -14,16 +14,14 @@
 (* limitations under the License.                                           *)
 (****************************************************************************)
 
+Require Import Coq.Lists.List.
 Require Import Coq.NArith.NArith.
+Require Import Coq.ZArith.ZArith.
+Import ListNotations.
 Local Open Scope N_scope.
 
 (* Specification of SHA-256 as described by FIPS 180-4:
    https://nvlpubs.nist.gov/nistpubs/FIPS/NIST.FIPS.180-4.pdf  *)
-
-(* Notations for bitwise operations, all left-associative *)
-Local Infix "<<" := N.shiftl (at level 32, left associativity, only parsing).
-Local Infix ">>" := N.shiftr (at level 32, left associativity, only parsing).
-Local Infix "⊕" := N.lxor (at level 32, left associativity, only parsing).
 
 (* Word size for SHA-256 *)
 Definition w := 32.
@@ -31,13 +29,28 @@ Definition w := 32.
 (* Addition of w-bit words *)
 Definition add_mod (x y : N) := (x + y) mod (2 ^ w).
 
+(* Truncating shift-left *)
+Definition truncating_shiftl (x n : N) := (N.shiftl x n) mod (2 ^ w).
+
+(* Notations for bitwise operations as defined in section 2.2.2, all
+   left-associative *)
+Local Infix "<<" := truncating_shiftl (at level 32, left associativity, only parsing).
+Local Infix ">>" := N.shiftr (at level 32, left associativity, only parsing).
+Local Infix "|" := N.lor (at level 32, left associativity, only parsing).
+Local Infix "&" := N.land (at level 32, left associativity, only parsing).
+Local Infix "⊕" := N.lxor (at level 32, left associativity, only parsing).
+Local Notation "¬ x" := (N.lnot x w) (at level 32, only parsing).
+
+(* All addition henceforth is add_mod *)
+Local Infix "+" := add_mod (at level 50, left associativity, only parsing).
+
 (* From section 2.2.2:
 
    The rotate right (circular right shift) operation, where x is a w-bit word
    and n is an integer with 0 <= n < w, is defined by
        ROTR n x = (x >> n) ∨ (x << w - n).
  *)
-Definition ROTR n x := N.lor (x >> n) (x << (w - n)).
+Definition ROTR n x := (x >> n) | (x << (w - n)).
 
 (* From section 2.2.2:
 
@@ -45,13 +58,11 @@ Definition ROTR n x := N.lor (x >> n) (x << (w - n)).
    0 <= n < w, is defined by SHR n x = x >> n. *)
 Definition SHR n x := x >> n.
 
-(* Six logical functions from section 4.1.2 *)
-
 (* Equation 4.2: Ch(x,y,z) = (x ^ y) ⊕ (¬ x ^ z) *)
-Definition Ch (x y z : N) := (N.land x y) ⊕ (N.land (N.lnot x w) z).
+Definition Ch (x y z : N) := (x & y) ⊕ ((¬ x) & z).
 
 (* Equation 4.3: Maj(x, y,z) = (x ^ y) ⊕ (x ^ z) ⊕ (y ^ z) *)
-Definition Maj (x y z : N) := (N.land x y) ⊕ (N.land x z) ⊕ (N.land y z).
+Definition Maj (x y z : N) := (x & y) ⊕ (x & z) ⊕ (y & z).
 
 (* Equation 4.4: Σ{0,256} (x) = (ROTR 2 x) ⊕ (ROTR 13 x) ⊕ (ROTR 22 x) *)
 Definition Sigma0 (x : N) := (ROTR 2 x) ⊕ (ROTR 13 x) ⊕ (ROTR 22 x).
@@ -64,3 +75,167 @@ Definition sigma0 (x : N) := (ROTR 7 x) ⊕ (ROTR 18 x) ⊕ (SHR 3 x).
 
 (* Equation 4.7: σ{1,256} (x) = (ROTR 17 x) ⊕ (ROTR 19 x) ⊕ (SHR 10 x) *)
 Definition sigma1 (x : N) := (ROTR 17 x) ⊕ (ROTR 19 x) ⊕ (SHR 10 x).
+
+(* From section 4.2.2:
+
+   SHA-224 and SHA-256 use the same sequence of sixty-four constant 32-bit
+   words, K{0,256},K{1,256}, ...K{63,256}. These words represent the first
+   thirty-two bits of the fractional parts of the cube roots of the first
+   sixty-four prime numbers. In hex, these constant words are (from left to
+   right):
+
+   428a2f98 71374491 b5c0fbcf e9b5dba5 3956c25b 59f111f1 923f82a4 ab1c5ed5
+   d807aa98 12835b01 243185be 550c7dc3 72be5d74 80deb1fe 9bdc06a7 c19bf174
+   e49b69c1 efbe4786 0fc19dc6 240ca1cc 2de92c6f 4a7484aa 5cb0a9dc 76f988da
+   983e5152 a831c66d b00327c8 bf597fc7 c6e00bf3 d5a79147 06ca6351 14292967
+   27b70a85 2e1b2138 4d2c6dfc 53380d13 650a7354 766a0abb 81c2c92e 92722c85
+   a2bfe8a1 a81a664b c24b8b70 c76c51a3 d192e819 d6990624 f40e3585 106aa070
+   19a4c116 1e376c08 2748774c 34b0bcb5 391c0cb3 4ed8aa4a 5b9cca4f 682e6ff3
+   748f82ee 78a5636f 84c87814 8cc70208 90befffa a4506ceb bef9a3f7 c67178f2
+ *)
+Definition K : list N :=
+  [ 0x428a2f98; 0x71374491; 0xb5c0fbcf; 0xe9b5dba5; 0x3956c25b; 0x59f111f1; 0x923f82a4; 0xab1c5ed5;
+    0xd807aa98; 0x12835b01; 0x243185be; 0x550c7dc3; 0x72be5d74; 0x80deb1fe; 0x9bdc06a7; 0xc19bf174;
+    0xe49b69c1; 0xefbe4786; 0x0fc19dc6; 0x240ca1cc; 0x2de92c6f; 0x4a7484aa; 0x5cb0a9dc; 0x76f988da;
+    0x983e5152; 0xa831c66d; 0xb00327c8; 0xbf597fc7; 0xc6e00bf3; 0xd5a79147; 0x06ca6351; 0x14292967;
+    0x27b70a85; 0x2e1b2138; 0x4d2c6dfc; 0x53380d13; 0x650a7354; 0x766a0abb; 0x81c2c92e; 0x92722c85;
+    0xa2bfe8a1; 0xa81a664b; 0xc24b8b70; 0xc76c51a3; 0xd192e819; 0xd6990624; 0xf40e3585; 0x106aa070;
+    0x19a4c116; 0x1e376c08; 0x2748774c; 0x34b0bcb5; 0x391c0cb3; 0x4ed8aa4a; 0x5b9cca4f; 0x682e6ff3;
+    0x748f82ee; 0x78a5636f; 0x84c87814; 0x8cc70208; 0x90befffa; 0xa4506ceb; 0xbef9a3f7; 0xc67178f2 ].
+
+(* From section 5.3.3:
+
+   For SHA-256, the initial hash value, H(0), shall consist of the following eight
+   32-bit words, in hex:
+
+   H0(0) = 6a09e667
+   H1(0) = bb67ae85
+   H2(0) = 3c6ef372
+   H3(0) = a54ff53a
+   H4(0) = 510e527f
+   H5(0) = 9b05688c
+   H6(0) = 1f83d9ab
+   H7(0) = 5be0cd19
+ *)
+Definition H0 : list N :=
+  [ 0x6a09e667
+    ; 0xbb67ae85
+    ; 0x3c6ef372
+    ; 0xa54ff53a
+    ; 0x510e527f
+    ; 0x9b05688c
+    ; 0x1f83d9ab
+    ; 0x5be0cd19 ].
+
+Section WithMessage.
+  Context (l msg : N). (* l = message length in bits *)
+
+  (* From section 5.1.1:
+
+     Suppose that the length of the message, M, is l bits. Append the bit “1” to
+     the end of the message, followed by k zero bits, where k is the smallest,
+     non-negative solution to the equation (l + 1 + k = 448) (mod 512). Then
+     append the 64-bit block that is equal to the number l expressed using a
+     binary representation.
+   *)
+  (* N.B. calculation of k is done in Z to avoid subtraction underflow *)
+  Definition k := Z.to_N ((448 - (Z.of_N l + 1)) mod 512)%Z.
+
+  (* N.B. Use N.shiftl here to avoid truncation *)
+  Definition padded_msg : N :=
+    (N.shiftl msg (N.add k 65)) | (N.shiftl 1 (N.add k 64)) | l.
+
+  (* Number of 512-bit blocks in padded message *)
+  Definition Nblocks : N := (N.add (N.add l k) 65) / 512.
+
+  (* From section 5.2.1:
+
+     For SHA-1, SHA-224 and SHA-256, the message and its padding are parsed into
+     N 512-bit blocks, M(1), M(2),...M(N). Since the 512 bits of the input block
+     may be expressed as sixteen 32- bit words, the first 32 bits of message
+     block i are denoted M0(i), M1(i), and so on up to M15(i).
+   *)
+  (* N.B. FIPS is using a big-endian convention when splitting the 512 bits into
+  32-bit blocks *)
+  Definition M (j i : N) :=
+    let Mi := (padded_msg >> (512*i)) mod (2^512) in
+    (Mi >> (32*(15-j))) mod (2^32).
+
+  (* From section 6.2.2 (step 1):
+
+     Prepare the message schedule, {W(t)}:
+     W(t) = Mt(i) for 0 <= t <= 15
+     W(t) = σ{1,256}(W_(t-2)) + W(t-7) + σ{0,256}(W(t-15)) + W(t-16) for 16 <= t <= 63
+   *)
+  Definition W (i : N) : list N :=
+    fold_left (fun (W : list N) t =>
+                 let wt :=
+                     if (t <? 16)%nat
+                     then M (N.of_nat t) i
+                     else
+                       let W_tm2 := nth (t-2) W 0 in
+                       let W_tm7 := nth (t-7) W 0 in
+                       let W_tm15 := nth (t-15) W 0 in
+                       let W_tm16 := nth (t-16) W 0 in
+                       (sigma1 W_tm2) + W_tm7 + (sigma0 W_tm15) + W_tm16 in
+                 W ++ [wt])
+              (seq 0 64) [].
+
+  (* See steps in section 6.2.2. *)
+  Definition sha256_step
+             (H : list N) (i : nat) : list N :=
+    (* step 2 : initialize working variables *)
+    let a := nth 0 H 0 in
+    let b := nth 1 H 0 in
+    let c := nth 2 H 0 in
+    let d := nth 3 H 0 in
+    let e := nth 4 H 0 in
+    let f := nth 5 H 0 in
+    let g := nth 6 H 0 in
+    let h := nth 7 H 0 in
+
+    (* step 3 : loop *)
+    let '(a,b,c,d,e,f,g,h) :=
+        fold_left
+          (fun '(a,b,c,d,e,f,g,h) t =>
+             let Kt := nth t K 0 in
+             let Wt := nth t (W (N.of_nat i)) 0 in
+             let T1 := h + (Sigma1 e) + (Ch e f g) + Kt + Wt in
+             let T2 := (Sigma0 a) + (Maj a b c) in
+             let h := g in
+             let g := f in
+             let f := e in
+             let e := d + T1 in
+             let d := c in
+             let c := b in
+             let b := a in
+             let a := T1 + T2 in
+             (a,b,c,d,e,f,g,h))
+          (seq 0 64)
+          (a,b,c,d,e,f,g,h) in
+
+    (* step 4 : get ith intermediate hash value *)
+    [ a + (nth 0 H 0)
+      ; b + (nth 1 H 0)
+      ; c + (nth 2 H 0)
+      ; d + (nth 3 H 0)
+      ; e + (nth 4 H 0)
+      ; f + (nth 5 H 0)
+      ; g + (nth 6 H 0)
+      ; h + (nth 7 H 0) ].
+
+  (* Concatenate the w-bit words of the hash value to get the full digest *)
+  Definition concat_digest (H : list N) :=
+    fold_left (fun D Hi => (N.shiftl D w) | Hi) H 0.
+
+  (* Full SHA-256 computation: loop of sha256_step *)
+  Definition sha256 :=
+    let n := N.to_nat Nblocks in
+    let H := fold_left sha256_step (seq 0 n) H0 in
+    concat_digest H.
+End WithMessage.
+
+(* Test vector from https://csrc.nist.gov/CSRC/media/Projects/Cryptographic-Standards-and-Guidelines/documents/examples/SHA256.pdf *)
+Goal (let abc := ((97 << 16) | (98 << 8) | 99) in
+      sha256 24 abc = 0xba7816bf8f01cfea414140de5dae2223b00361a396177a9cb410ff61f20015ad).
+Proof. vm_compute. reflexivity. Qed.
